backend/RTLExtra.v
@@ -40,6 +40,11 @@ Definition regset_inject_incr F1 F2 rs trs
   regset_inject F2 rs trs.
 Proof. ii. eapply val_inject_incr; eauto. Qed.
 
+Lemma regset_inject_val_inject F rs trs r
+      (INJ: regset_inject F rs trs):
+  val_inject F rs # r trs # r.
+Proof. auto. Qed.
+
 Lemma regset_inject_val_list_inject F rs trs l
       (INJ: regset_inject F rs trs):
   val_list_inject F rs ## l trs ## l.
@@ -142,96 +147,6 @@ Proof.
     eapply external_call_symbols_preserved; eauto.
   - eapply exec_Icond; eauto.
   - eapply exec_Ijumptable; eauto.
-Qed.
-
-Lemma is_normal_inject
-      ge s f sp pc1 rs1 m1 pc2 rs2 m2 tr
-      tge ts tsp trs1 tm1
-      F1
-      (SYMBOL: forall (s: ident), Genv.find_symbol tge s = Genv.find_symbol ge s)
-      (VARINFO: forall b, Genv.find_var_info tge b = Genv.find_var_info ge b)
-      (NORMAL1: is_normal (State s f (Vptr sp Int.zero) pc1 rs1 m1))
-      (STEP: step ge (State s f (Vptr sp Int.zero) pc1 rs1 m1) tr (State s f (Vptr sp Int.zero) pc2 rs2 m2))
-      (SP: F1 sp = Some(tsp, 0))
-      (PRES1: meminj_preserves_globals ge F1)
-      (REGSET1: regset_inject F1 rs1 trs1)
-      (MEM1: Mem.inject F1 m1 tm1):
-  exists F2 trs2 tm2,
-    <<TSTEP: step tge (State ts f (Vptr tsp Int.zero) pc1 trs1 tm1) tr (State ts f (Vptr tsp Int.zero) pc2 trs2 tm2)>> /\
-    <<MAXPERM: forall b ofs p, Mem.valid_block m1 b -> Mem.perm m2 b ofs Max p -> Mem.perm m1 b ofs Max p>> /\
-    <<MAXPERM': forall b ofs p, Mem.valid_block tm1 b -> Mem.perm tm2 b ofs Max p -> Mem.perm tm1 b ofs Max p>> /\
-    <<UNCHANGED: Mem.unchanged_on (loc_out_of_reach F1 m1) tm1 tm2>> /\
-    <<REGSET2: regset_inject F2 rs2 trs2>> /\
-    <<MEM2: Mem.inject F2 m2 tm2>> /\
-    <<INCR: inject_incr F1 F2>> /\
-    <<SEP: inject_separated F1 F2 m1 tm1>>.
-Proof.
-  simpl in *. destruct (fn_code f) ! pc1 as [[]|] eqn:X; clarify; inv STEP; clarify.
-  - eexists. eexists. eexists. splits; eauto.
-    + apply exec_Inop; eauto.
-    + apply Mem.unchanged_on_refl.
-    + apply inject_separated_refl.
-  - exploit eval_operation_inject; try apply H10; eauto.
-    { apply regset_inject_val_list_inject. eauto. }
-    rewrite shift_stack_operation_Int_zero. intro. des.
-    eexists. eexists. eexists. splits; eauto.
-    + eapply exec_Iop; eauto.
-      erewrite eval_operation_preserved; eauto.
-    + apply Mem.unchanged_on_refl.
-    + apply regset_inject_set_reg; auto.
-    + apply inject_separated_refl.
-  - exploit eval_addressing_inject; try apply H10; eauto.
-    { apply regset_inject_val_list_inject. eauto. }
-    rewrite shift_stack_addressing_Int_zero. intro. des.
-    exploit Mem.loadv_inject; eauto.
-    intro. des.
-    eexists. eexists. eexists. splits; eauto.
-    + eapply exec_Iload; eauto.
-      erewrite eval_addressing_preserved; eauto.
-    + apply Mem.unchanged_on_refl.
-    + apply regset_inject_set_reg; auto.
-    + apply inject_separated_refl.
-  - exploit eval_addressing_inject; try apply H10; eauto.
-    { apply regset_inject_val_list_inject. eauto. }
-    rewrite shift_stack_addressing_Int_zero. intro. des.
-    exploit Mem.storev_mapped_inject; eauto.
-    intro. des.
-    eexists. eexists. exists n2. splits; eauto.
-    + eapply exec_Istore; eauto.
-      erewrite eval_addressing_preserved; eauto.
-    + destruct a0; inv H11. intros. eapply Mem.perm_store_2; eauto.
-    + destruct v2; inv H1. intros. eapply Mem.perm_store_2; eauto.
-    + destruct v2; inv H1. eapply Mem.store_unchanged_on; eauto. ii.
-      inv H0; [|inv H11]. simpl in *.
-      exploit Mem.store_valid_access_3; try apply H11; eauto. intros VA1.
-      exploit Mem.store_valid_access_1; try apply H11; eauto. intros VA2.
-      destruct VA1 as [PERM1 _], VA2 as [PERM2 _].
-      erewrite Mem.address_inject in H1; eauto.
-      * eapply H3; eauto.
-        apply Mem.perm_cur_max. eapply Mem.perm_implies; [|apply perm_any_N]. apply PERM1. xomega.
-      * apply PERM2. xomega.
-    + apply inject_separated_refl.
-  - exploit external_call_mem_inject; eauto.
-    { apply regset_inject_val_list_inject. eauto. }
-    intro. des. eexists. eexists. eexists. splits; try apply H1; eauto.
-    + econs; eauto.
-      eapply external_call_symbols_preserved; eauto. 
-    + intros. eapply external_call_max_perm; eauto.
-    + intros. eapply external_call_max_perm; eauto.
-    + apply regset_inject_set_reg; auto.
-      eapply regset_inject_incr; eauto.
-  - exploit eval_condition_inject; try apply H10; eauto.
-    { apply regset_inject_val_list_inject. eauto. }
-    intro.
-    eexists. eexists. eexists. splits; eauto.
-    + eapply exec_Icond; eauto.
-    + apply Mem.unchanged_on_refl.
-    + apply inject_separated_refl.
-  - eexists. eexists. eexists. splits; eauto.
-    + eapply exec_Ijumptable; eauto.
-      generalize (REGSET1 r). rewrite H10. intro X. inv X. auto.
-    + apply Mem.unchanged_on_refl.
-    + apply inject_separated_refl.
 Qed.
 
 Lemma is_normal_extends
